using the default libary for permutation, sorting, have the cmp_of_rel to covering total ordering on all number.

work-in-progress/sorting/SortingLB.ec
@@ -19,7 +19,7 @@ timeout 2.  (* can increase *)
    the jth element (the answer is true or false); it can't ask
    questions about the values of the list elements themselves *)
 
-require import AllCore List IntDiv StdOrder IntMin FSetAux.
+require import AllCore List IntDiv StdOrder IntMin FSetAux Perms Binomial.
 import IntOrder.
 
 require AdvLowerBounds.   (* adversarial lower bounds framework *)
@@ -177,367 +177,87 @@ type aux = unit.  (* no auxiliary information *)
 op good (aux : aux, xs : inp list) : bool =
   total_ordering xs.
 
-op elems_in_range (ms : int list, n : int) : bool =
-  forall (i : int),
-  0 <= i < size ms => 0 <= nth witness ms i < n.
+  (* sort with total ordering*)
 
-lemma nth_cons0 (x : 'a, ys : 'a list) :
-  nth witness (x :: ys) 0 = x.
-proof. trivial. qed.
+op cmp_of_rel (xs: inp list) (x , y : int) : bool =
+  if (0 <= x < len /\ 0 <= y < len)
+  then rel xs x y
+  else  if (0 <= x < len) then true
+  else  if (0 <= y < len) then false
+  else  x <= y.
 
-lemma nth_cons_pos (x : 'a, ys : 'a list, i : int) :
-  0 <= i < size ys =>
-  nth witness (x :: ys) (i + 1) = nth witness ys i.
-proof. smt(). qed.
-
-lemma elems_in_range0 (n : int) :
-  elems_in_range [] n.
-proof. smt(). qed.
-
-lemma elems_in_range1 (m n : int) :
-  0 <= m < n => elems_in_range [m] n.
-proof. rewrite /elems_in_range /#. qed.
-
-lemma elems_in_range_cons (m : int, ms : int list, n : int) :
-  elems_in_range (m :: ms) n <=>
-  0 <= m < n /\ elems_in_range ms n.
-proof.
-rewrite /elems_in_range.
-split => [H | /#].
-split.
-rewrite -(nth_cons0 m ms) H; smt(size_ge0).
-move => i [ge0_i lt_i_size_ms].
-rewrite -(nth_cons_pos m ms) // H /#.
-qed.
-
-lemma elems_in_range_incr (ms : int list, n : int) :
-  elems_in_range ms n => elems_in_range ms (n + 1).
-proof. smt(). qed.
-
-op nodups (xs : 'a list) : bool =  (* like uniq but using nth *)
+op nosmt cmp_total_ordering (xs: inp list) : bool =
+  size xs = arity /\
+  (forall (i : int), cmp_of_rel xs i i) /\
+  (forall (i j k : int),
+    cmp_of_rel xs i j => cmp_of_rel xs j k => cmp_of_rel xs i k) /\
+  (forall (i j : int),
+    cmp_of_rel xs i j => cmp_of_rel xs j i => i = j) /\
   forall (i j : int),
-  0 <= i < j < size xs => nth witness xs i <> nth witness xs j.
+    i <> j => cmp_of_rel xs i j \/ cmp_of_rel xs j i.
 
-lemma nodups0 :
-  nodups <:'a>[].
-proof. smt(). qed.
+lemma cmp_total_ordering_size (xs : inp list) :
+  cmp_total_ordering xs => size xs = arity.
+proof. rewrite /cmp_total_ordering /#. qed.
 
-lemma nodups_cons_def (x : 'a, ys : 'a list) :
-  nodups (x :: ys) <=>
-  nodups ys /\
-  (forall (i : int), 0 <= i < size ys => nth witness ys i <> x).
+lemma cmp_total_ordering_refl (xs : inp list, i : int) :
+  cmp_total_ordering xs  => cmp_of_rel xs i i.
+proof. rewrite /cmp_total_ordering /#. qed.
+
+lemma cmp_total_ordering_trans (xs : inp list, j i k : int) :
+  cmp_total_ordering xs =>
+  cmp_of_rel xs i j => cmp_of_rel xs j k => cmp_of_rel xs i k.
+proof. rewrite /cmp_total_ordering /#. qed.
+
+lemma cmp_total_ordering_antisym (xs : inp list, i j : int) :
+  cmp_total_ordering xs =>
+  cmp_of_rel xs i j => cmp_of_rel xs j i => i = j.
+proof. rewrite /cmp_total_ordering /#. qed.
+
+lemma cmp_total_ordering_total (xs : inp list, i j : int) :
+  cmp_total_ordering xs =>
+  cmp_of_rel xs i j \/ cmp_of_rel xs j i.
+proof. rewrite /cmp_total_ordering /#. qed.
+
+lemma cmp_total_ordering_ne_not_sym (xs : inp list, i j : int) :
+  cmp_total_ordering xs =>
+   i <> j =>
+  cmp_of_rel xs i j => ! cmp_of_rel xs j i.
+proof. rewrite /cmp_total_ordering /#. qed.
+  
+
+lemma tot_cmp_tot (xs:inp list):
+    total_ordering xs => cmp_total_ordering (xs).
 proof.
-rewrite /nodups.
-split => [H | /#].
-split => [i j [#] ge0_i lt_i_j lt_j_size_ys |].
-rewrite -(nth_cons_pos x) 1:/# -(nth_cons_pos x ys) 1:/# 1:H /= /#.
-move => i [ge0_i lt_i_size_ys].
-rewrite eq_sym -(nth_cons0 _ ys) -(nth_cons_pos x ys) 1:/# H /#.
-qed.
+  rewrite /cmp_total_ordering /total_ordering => //.
+  smt().
+qed.    
 
-(* tests whether xs is a permutation of the elements 0 ... n - 1: *)
+op tsort (xs: inp list) (s: int list) =
+   sort ( cmp_of_rel xs  ) s.
 
-op is_perm (n : int, xs : int list) : bool =
-  size xs = n /\ elems_in_range xs n /\ nodups xs.
+op tsorted (xs: inp list) (s: int list) =
+   sorted ( cmp_of_rel xs ) s.
 
-lemma perm_has_all (n : int, xs : int list, i : int) :
-  is_perm n xs => 0 <= i < n =>
-  exists (j : int), 0 <= j < n /\ nth witness xs j = i.
-proof.  
-have H :
-  forall (n : int),
-  0 <= n =>
-  forall (xs : int list),
-  is_perm n xs =>
-  (forall (i : int),
-   0 <= i < n =>
-   exists (j : int), 0 <= j < n /\ nth witness xs j = i).
-  clear n xs i.
-  elim => [xs _ i [ge0_i lt0_i] | n ge0_n IH xs].
-  have // : 0 < 0 by rewrite (ler_lt_trans i).
-  rewrite /is_perm /elems_in_range =>
-    [[#] size_xs all_xs_in_rng no_dups_xs i [ge0_i lt_i_n_plus1]].
-  rewrite size_xs in all_xs_in_rng.
-  case (exists j, 0 <= j < n + 1 /\ nth witness xs j = n) =>
-    [[j [#] ge0_j lt_j_n_plus1 jth_xs_eq_n] | all_xs_ne_n].
-  case (i = n) => [eq_i_n | ne_i_n].
-  exists j; smt().
-  have [k [#] ge0_k lt_k_n <-] := IH (trim xs j) _ i _.
-    rewrite /is_perm /elems_in_range /=.
-    split; first smt(size_trim).
-    rewrite /trim.
-    smt(nth_cat size_cat size_take size_drop nth_take nth_drop).
-    smt().
-  rewrite /trim nth_cat size_take // size_xs lt_j_n_plus1 /=.
-  case (k < j) => [lt_k_j | not_lt_k_j].
-  exists k; smt(nth_take).
-  exists (k + 1); smt(nth_drop).
-  rewrite negb_exists /= in all_xs_ne_n.
-  have ge0_hd_xs_lt_n : 0 <= head witness xs < n by smt(nth0_head).
-  have [j [#] ge0_j lt_j_n jth_behead_xs_eq_head_xs]
-         := IH (behead xs) _ (head witness xs) _.
-    rewrite /is_perm /nodups.
-    smt(nth_behead head_behead).
-    trivial.
-  have /# :  (* contradiction *)
-       exists (i j : int),
-       0 <= i < j < n + 1 /\ nth witness xs i = nth witness xs j.
-    exists 0 (j + 1); smt(nth0_head nth_behead).
-move => is_perm_gne_n_xs [ge0_i lt_i_n].
-by rewrite H 1:(ler_trans i) // ltrW.
-qed.
-
-(* tests whether xs is a permutation of the elements 0 ... len - 1: *)
-
-op is_perm_len : int list -> bool = is_perm len.
-
-lemma perm_len_has_all (xs : int list, i : int) :
-  is_perm_len xs => 0 <= i < len =>
-  exists (j : int), 0 <= j < len /\ nth witness xs j = i.
-proof. apply perm_has_all. qed.
-
-(* assuming total_ordering xs and elems_in_range ms len: *)
-
-op sorted (xs : inp list, ms : int list) : bool =
-  forall (i j : int),
-  0 <= i <= j < size ms =>
-  rel xs (nth witness ms i) (nth witness ms j).
-
-lemma sorted0 (xs : inp list) :
-  sorted xs [].
-proof. smt(). qed.
-
-lemma sorted1 (xs : inp list, m : int) :
-  total_ordering xs => 0 <= m < len => sorted xs [m].
-proof.
-move => tot_ord_xs [ge0 lt_m_len].
-rewrite /sorted.
-smt(total_ordering_refl).
-qed.
-
-lemma sorted_cons_def (xs : inp list, m : int, ms : int list) :
-  total_ordering xs =>
-  sorted xs (m :: ms) /\ elems_in_range (m :: ms) len <=>
-  (ms = [] /\ 0 <= m < len \/
-   ms <> [] /\ 0 <= m < len /\ rel xs m (head witness ms) /\
-   sorted xs ms /\ elems_in_range ms len).
-proof.
-move => tot_ord_xs.
-split =>
-  [[srtd_m_ms eir_m_ms] |
-   [[#] -> ge0_m lt_m_len |
-    [#] ge0_m lt_m_len ms_nonnil rel_xs_m_hd_ms srtd_xs_ms eir_ms]].
-case (ms = []) => [_ /= | /= ms_nonnil].
-smt(elems_in_range_cons).
-split; first smt(elems_in_range_cons).
-split.
-have -> : m = nth witness (m :: ms) 0 by smt().
-have -> : head witness ms = nth witness (m :: ms) 1.
-  by rewrite /= nth0_head.
-rewrite srtd_m_ms /=.
-smt(size_ge0 size_eq0).
-split => [i j [#] ge0_i le_i_j lt_j_size_ms |].
-have -> : nth witness ms i = nth witness (m :: ms) (i + 1) by smt().
-have -> : nth witness ms j = nth witness (m :: ms) (j + 1) by smt().
-rewrite srtd_m_ms /#.
-smt(elems_in_range_cons).
-by rewrite sorted1 //= elems_in_range1.
-split.
-move => i j [#] /= ge0_i le_i_j lt_j_size_ms_plus1.
-case (i = 0) => [eq0_i | ne0_i].
-case (j = 0) => [eq0_j | ne0_j].
-by rewrite total_ordering_refl.
-rewrite (total_ordering_trans xs (head witness ms)) //.
-smt(nth0_head).
-smt().
-smt(nth0_head).
-smt().
-smt(elems_in_range_cons).
-qed.
-
-lemma sorted_cons_nonempty (xs : inp list, m : int, ms : int list) :
-  total_ordering xs => 0 <= m < len => ms <> [] =>
-  elems_in_range ms len => rel xs m (head witness ms) => sorted xs ms =>
-  sorted xs (m :: ms).
-proof. smt(sorted_cons_def). qed.
-
-lemma sorted_cons_nonempty_rel (xs : inp list, m : int, ms : int list) :
-  ms <> [] => sorted xs (m :: ms) =>
-  rel xs m (head witness ms).
-proof.
-move => ms_nonnil srtd_m_ms.
-have -> : m = nth witness (m :: ms) 0 by smt().
-have -> : head witness ms = nth witness (m :: ms) 1.
-  by rewrite /= nth0_head.
-rewrite srtd_m_ms /=.
-smt(size_ge0 size_eq0).
-qed.
-
-op insert_in_sorted (xs : inp list, n : int, ms : int list) : int list =
-  with ms = []      => [n]
-  with ms = l :: ls =>
-    if rel xs n l
-    then n :: ms
-    else l :: insert_in_sorted xs n ls.
-
-lemma insert_in_sorted_size (xs : inp list, n : int, ms : int list) :
-  size (insert_in_sorted xs n ms) = size ms + 1.
-proof. elim ms; smt(). qed.
-
-lemma insert_in_sorted_nonnil (xs : inp list, n : int, ms : int list) :
-  insert_in_sorted xs n ms <> [].
-proof. smt(insert_in_sorted_size size_eq0). qed.
-
-lemma insert_in_sorted_head (xs : inp list, n : int, ms : int list) :
-  ms <> [] /\
-  head witness (insert_in_sorted xs n ms) = head witness ms \/
-  head witness (insert_in_sorted xs n ms) = n.
-proof.
-case ms => [// | m ms /=].
-by case (rel xs n m).
-qed.
-
-lemma insert_in_sorted_elems_in_range_gen
-      (len' : int, xs : inp list, n : int, ms : int list) :
-  1 <= len' => total_ordering xs =>
-  0 <= n < len' => elems_in_range ms len' =>
-  elems_in_range (insert_in_sorted xs n ms) len'.
-proof.
-move => ge1_len' tot_ord_xs [ge0_n lt_n_len'].
-elim ms => [/= | l ls IH /= eir_ls].
-rewrite /elems_in_range /#.
-case (rel xs n l) => [rel_xs_n_l | not_rel_xs_n_l].
-by rewrite elems_in_range_cons.
-rewrite elems_in_range_cons.
-split; first smt(elems_in_range_cons).
-rewrite IH.
-smt(elems_in_range_cons).
-qed.
-
-lemma insert_in_sorted_elems_in_range
-      (xs : inp list, n : int, ms : int list) :
-  total_ordering xs => 0 <= n < len => elems_in_range ms len =>
-  elems_in_range (insert_in_sorted xs n ms) len.
-proof.
-apply insert_in_sorted_elems_in_range_gen.
-rewrite ge1_len.
-qed.
-
-op all_nth_ne (l : 'a, ms : 'a list) : bool =
-  forall (i : int),
-  0 <= i < size ms => nth witness ms i <> l.
-
-lemma insert_in_sorted_not_elem_nth
-      (xs : inp list, k n : int, ms : int list) :
-  total_ordering xs => k <> n => all_nth_ne k ms =>
-  all_nth_ne k (insert_in_sorted xs n ms).
-proof.
-move => tot_ord_xs ne_k_n.
-rewrite /all_nth_ne.
-elim ms => [/# | l ls IH k_not_in_l_ls i].
-rewrite insert_in_sorted_size /= => [[ge0_i lt_i_size_ls_plus2]]. 
-case (rel xs n l) => [rel_xs_n_l | not_rel_xs_n_l].
-case (i = 0) => [/# | ne0_i].
-case (i - 1 = 0) => [eq0_i_min1 | ne0_i_min1].
-have -> : l = nth witness (l :: ls) 0 by smt().
-rewrite k_not_in_l_ls /=; smt(size_ge0).
-have -> :
-  nth witness ls (i - 1 - 1) = nth witness (l :: ls) (i - 1)
-  by smt().
-rewrite k_not_in_l_ls /=; smt(size_ge0).
-case (i = 0) => [eq0_i | ne0_i].
-have -> : l = nth witness (l :: ls) 0 by smt().
-rewrite k_not_in_l_ls /=; smt(size_ge0).
-apply IH.
-move => j [ge0_j lt_j_size_ls].
-have -> : nth witness ls j = nth witness (l :: ls) (j + 1) by smt().
-rewrite k_not_in_l_ls //=; smt(size_ge0).
-rewrite insert_in_sorted_size; smt(size_ge0).
-qed.
-
-lemma insert_in_sorted_no_dups (xs : inp list, n : int, ms : int list) :
-  total_ordering xs => all_nth_ne n ms =>  
-  nodups ms => nodups (insert_in_sorted xs n ms).
-proof.
-move => tot_ord_xs.
-elim ms => [/= _ | l ls IH n_not_in_l_ls nodups_l_ls /=].
-smt().
-case (rel xs n l) => [rel_xs_n_l | not_rel_xs_n_l].
-rewrite nodups_cons_def.
-split; first rewrite nodups_l_ls.
-move => i [ge0_i lt_i_size_l_ls].
-by rewrite n_not_in_l_ls.
-rewrite nodups_cons_def.
-split.
-rewrite IH => [i [ge0_i lt_i_size_ls] |].
-have -> : nth witness ls i = nth witness (l :: ls) (i + 1) by smt().
-rewrite n_not_in_l_ls /#.
-smt(nodups_cons_def).
-apply insert_in_sorted_not_elem_nth => //.
-have -> : l = nth witness (l :: ls) 0 by smt().
-rewrite n_not_in_l_ls //=; smt(size_ge0).
-smt(nodups_cons_def).
-qed.
-
-lemma insert_in_sorted_perm_gen (xs : inp list, n : int, ms : int list) :
-  total_ordering xs => 0 <= n < len => is_perm n ms =>
-  is_perm (n + 1) (insert_in_sorted xs n ms).
-proof.
-move => tot_ord_xs [ge0_n lt_n_len].
-rewrite /is_perm => [#] size_ms_eq_n eir_ms_n no_dups_ms.
-split; first rewrite insert_in_sorted_size /#.
-split.
-by rewrite insert_in_sorted_elems_in_range_gen // 1:/# 1:/#
-           elems_in_range_incr.
-rewrite insert_in_sorted_no_dups // /#.
-qed.
-
-lemma insert_in_sorted_sorted (xs : inp list, n : int, ms : int list) :
-  total_ordering xs => 0 <= n < len => elems_in_range ms len =>
-  sorted xs ms => sorted xs (insert_in_sorted xs n ms).
-proof.
-move => tot_ord_xs.
-elim ms =>
-  [[ge0_n lt_n_len] _ _ /= |
-   m ms IH lt_n_len range_m_ms sorted_m_ms /=].
-by rewrite sorted1.
-case (rel xs n m) => [rel_xs_n_m | not_rel_xs_n_m].
-smt(sorted_cons_def).
-have ge0_m_lt_len : 0 <= m < len.
-  have -> : m = nth witness (m :: ms) 0 by trivial.
-  rewrite range_m_ms /=; smt(size_ge0).
-rewrite sorted_cons_nonempty //.
-by rewrite insert_in_sorted_nonnil.
-rewrite insert_in_sorted_elems_in_range //.
-smt(elems_in_range_cons).
-have [[ms_ne_nil ->] | ->] := insert_in_sorted_head xs n ms.
-by rewrite sorted_cons_nonempty_rel.
-smt(total_ordering_total).
-rewrite IH //.
-smt(elems_in_range_cons).
-smt(sorted_cons_def).
-qed.
 
 lemma sorted_perm_exists (xs : inp list) :
   total_ordering xs =>
   exists (perm : int list),
-  is_perm_len perm /\ sorted xs perm.
+  perm_eq (range 0 len) perm /\ tsorted xs perm.
 proof.
 move => tot_ord_xs.
 have H :
   forall (n : int),
   0 <= n => n <= len =>
   exists (perm : int list),
-  is_perm n perm /\ elems_in_range perm len /\ sorted xs perm.
-  elim => [_ | n ge0_n IH le_n_len].
-  exists []; smt().
-  have lt_n_len: n < len by smt().
-  have [perm [#] ip_n_perm eir_perm_len srtd_xs_perm] := IH _.
-    smt().
-  exists (insert_in_sorted xs n perm).
-  split; first by rewrite insert_in_sorted_perm_gen.
-  split; first by rewrite insert_in_sorted_elems_in_range.
-  by rewrite insert_in_sorted_sorted.
+  perm_eq (range 0 n) perm  /\ tsorted xs perm.
+  move => n ge0_n le_n_len.
+  exists (sort (cmp_of_rel xs) (range 0 (n))).
+  split.
+  smt(perm_eq_sym perm_sort).
+  rewrite /tsorted.
+  rewrite (sort_sorted).
+  smt(tot_cmp_tot cmp_total_ordering_total).
 have /# := H len _ _.
   rewrite (ler_trans 1) // ge1_len.
   trivial.
@@ -565,42 +285,9 @@ have /# := pmin_spec P _.
     trivial. smt().
 qed.
 
-lemma sorted_perm_uniq (xs : inp list, perm1 perm2 : int list) :
-  total_ordering xs =>
-  is_perm_len perm1 => is_perm_len perm2 =>
-  sorted xs perm1 => sorted xs perm2 =>
-  perm1 = perm2.
-proof.
-move => tot_ord_xs is1 is2 srted1 srted2.
-case (perm1 = perm2) => [// | ne_perms].
-have [i [#] ge0_i lt_i_size nth_ne_at_i min_prop]
-       := diff_equal_size_least_index_diff perm1 perm2 _ _.
-  smt(). smt().
-have [k1 [#] lt_i_k1 lt_k1_size perm1_at_k1_eq_perm2_at_i] :
-  exists (k1 : int),
-  i < k1 < size perm1 /\ nth witness perm1 k1 = nth witness perm2 i.
-  have [j [#] ge0_j lt_j_len perm1_at_j_eq_perm2_at_i]
-         := perm_len_has_all perm1 (nth witness perm2 i) _ _.
-    trivial. smt().
-  have i_lt_j_lt_len : i < j by smt().
-  exists j; smt().
-have [k2 [#] lt_i_k2 lt_k2_size perm2_at_k2_eq_perm1_at_i] :
-  exists (k2 : int),
-  i < k2 < size perm1 /\ nth witness perm2 k2 = nth witness perm1 i.
-  have [j [#] ge0_j lt_j_len perm2_at_j_eq_perm1_at_i]
-         := perm_len_has_all perm2 (nth witness perm1 i) _ _.
-    trivial. smt().
-  have i_lt_j_lt_len : i < j by smt().
-  exists j; smt().
-have rel_i_12 : rel xs (nth witness perm1 i) (nth witness perm2 i).
-  smt().
-have rel_i_21 : rel xs (nth witness perm2 i) (nth witness perm1 i).
-  smt().
-smt(total_ordering_ne_not_sym).
-qed.
 
 op sorted_perm_len_rel (xs : inp list, perm : int list) : bool =
-  is_perm_len perm /\ sorted xs perm.
+  perm_eq (range 0 len) perm /\ tsorted xs perm.
 
 lemma sorted_perm_rel_exists (xs : inp list) :
   total_ordering xs =>
@@ -612,8 +299,14 @@ lemma sorted_perm_len_rel_uniq (xs : inp list, perm1 perm2 : int list) :
   sorted_perm_len_rel xs perm1 => sorted_perm_len_rel xs perm2 =>
   perm1 = perm2.
 proof.
-move => tot_ord_xs [ispl1 srted1] [ispl2 srted2].
-by rewrite (sorted_perm_uniq xs perm1 perm2).
+move => tot_ord_xs [ispl1 srted1] [ispl2 srted2]. print eq_sorted.
+  rewrite (eq_sorted (cmp_of_rel xs) _ _ perm1 perm2).
+  smt(cmp_total_ordering_trans tot_cmp_tot).
+  smt(cmp_total_ordering_antisym tot_cmp_tot).
+  smt().
+  smt().
+  smt(perm_eq_trans perm_eq_sym).
+  trivial.
 qed.
 
 (* now we can define our f and show it has the correct property *)
@@ -622,18 +315,22 @@ type out = int list.
 
 op f (aux : aux, xs : inp list) : out option =
   if total_ordering xs
-  then Some (choiceb (sorted_perm_len_rel xs) [])
+  then Some (tsort xs (range 0 len) )
   else None.
 
 lemma f_prop (xs : inp list) :
   total_ordering xs =>
-  is_some (f () xs) /\ is_perm_len (oget (f () xs)) /\
-  sorted xs (oget (f () xs)).
+  is_some (f () xs) /\ perm_eq (range 0 len) (oget (f () xs)) /\
+  tsorted xs (oget (f () xs)).
 proof.
 move => tot_ord_xs.
-have := choicebP (sorted_perm_len_rel xs) [] _.
-  by rewrite sorted_perm_rel_exists.
-by rewrite /f /sorted_perm_len_rel tot_ord_xs.
+  split.
+  smt(sorted_perm_exists).
+  split.
+  rewrite /f /sorted_perm_len_rel tot_ord_xs => /=.
+  smt(perm_eq_sym perm_sort).
+  rewrite /tsort /f tot_ord_xs /tsorted /tsort => /=. 
+  smt(sort_sorted cmp_total_ordering_total tot_cmp_tot).
 qed.
 
 lemma f_is_some (xs : inp list) :
@@ -644,14 +341,14 @@ smt(f_prop).
 qed.
 
 lemma f_is_perm_len (xs : inp list) :
-  total_ordering xs => is_perm_len (oget (f () xs)).
+  total_ordering xs => perm_eq (range 0 len) (oget (f () xs)).
 proof.
 move => tot_ord_xs.
 smt(f_prop).
 qed.
 
 lemma f_sorted (xs : inp list) :
-  total_ordering xs => sorted xs (oget (f () xs)).
+  total_ordering xs => tsorted xs (oget (f () xs)).
 proof.
 move => tot_ord_xs.
 smt(f_prop).
@@ -690,5 +387,63 @@ have not_tot_ord_xs : ! total_ordering xs.
   elim.
   have // : all (mem univ) xs by smt(allP).
   by rewrite /good.
-smt(f_bad).
+  smt(f_bad).
+  qed.
 (* end of realization *)
+
+(* The adversary *)
+
+module Adv : ADV = {
+
+  var inpss : inp list list  (* current possible lists of inputs *)
+  
+  proc init() : unit = {
+    inpss <- init_inpss ();
+    return ();       
+  }
+
+  proc ans_query(i: int) : inp = {
+    (* var fst, snd : int ; *) (* stores the dec indices *)
+    var inpss_t, inpss_f : inp list list; (* two possible inpss sizes when the adversary answers true or false *) 
+    var ret : inp; 
+  
+    inpss_t <- (filter_nth inpss i true);
+    inpss_f <- (filter_nth inpss i false);      
+
+    if (size(inpss_t) <= size(inpss_f)){
+      inpss <- filter_nth inpss i false;  (*answering false remains more possible inpust*)
+      ret <- false;     
+      }
+    else {
+       (* this also covers:  1. the algorithm asks the rel of (i, i);
+                             2. (i, j) is asked before and this time (j, i);
+                             3. (i, j) = true, (j, k) = true,  this time asks (i,k), etc *)
+      inpss <- filter_nth inpss i true;  
+      ret <- true ;  
+    }
+    return ret;   
+  }
+}.    
+
+(* adversary is lossless *)
+
+lemma Adv_init_ll : islossless Adv.init.
+proof.
+proc; auto.
+qed.
+
+lemma Adv_ans_query_ll : islossless Adv.ans_query.
+proof.
+proc; auto.
+qed.
+
+
+
+(* here is our main theorem: *)
+
+lemma G_Adv_main (Alg <: ALG{Adv}) : 
+  hoare [G(Alg, Adv).main : true ==> res.`1 \/ int_log_up 2 (fact len) <= res.`2].
+proof.
+  admit.
+qed.
+    
